Prove (Next).nextTag_isSome_iff_queue_not_isEmpty

Runtime/Network/Execution/Next.lean
@@ -7,10 +7,54 @@ private def nextTime (exec : Executable net) : Option (Time.From exec.tag.time) 
   | none => none
   | some nextEvent => some ⟨nextEvent.time, exec.lawfulQueue h⟩
 
+theorem nextTime_isSome_iff_queue_not_isEmpty {exec : Executable net} : 
+  exec.nextTime.isSome ↔ ¬exec.queue.isEmpty := by
+  simp [Array.isEmpty, Option.isSome_def, nextTime]
+  constructor
+  case mp =>
+    intro ⟨_, h⟩ hc
+    split at h
+    · contradiction
+    case _ h' => 
+      simp [getElem?] at h'
+      split at h' 
+      case inl h => simp [hc] at h
+      case inr => contradiction
+  case mpr =>
+    intro h
+    let fst := exec.queue[0]' (Nat.zero_lt_of_ne_zero h)
+    by_cases exec.queue[0]? = some fst
+    case inl hc =>
+      have hq := exec.lawfulQueue hc
+      exists ⟨fst.time, hq⟩
+      split 
+      · simp_all [hc]
+      · simp_all
+    case inr hc =>
+      simp [getElem?] at hc
+      split at hc
+      case inl => contradiction
+      case inr => simp_all [Nat.zero_lt_of_ne_zero h]
+
 private def nextTag (exec : Executable net) : Option Tag := 
   match exec.nextTime with
   | none => none
   | some time => exec.tag.advance time
+
+theorem nextTag_isSome_iff_nextTime_isSome {exec : Executable net} :
+  exec.nextTag.isSome ↔ exec.nextTime.isSome := by
+  simp [nextTag]
+  split <;> simp [Option.isSome_def]
+  · intro ⟨_, _⟩; simp_all
+  case _ time _ =>
+    simp_all
+    constructor <;> intro _
+    · exists ‹_›
+    · exists exec.tag.advance time
+
+theorem nextTag_isSome_iff_queue_not_isEmpty {exec : Executable net} : 
+  exec.nextTag.isSome ↔ ¬exec.queue.isEmpty := by
+  simp [nextTag_isSome_iff_nextTime_isSome, nextTime_isSome_iff_queue_not_isEmpty]
 
 -- The first array are the next events to be executed at `time`.
 -- The second array is the remaining queue. 
@@ -19,36 +63,59 @@ private def eventSplit (exec : Executable net) (time : Time) : Array (Event net)
   let ⟨next, postponed⟩ := candidates.unique (·.id)
   (next, postponed ++ later)
 
+theorem eventSplit_fst_LawfulQueue {exec : Executable net} : 
+  LawfulQueue (exec.eventSplit time).fst time := sorry
+  -- TODO: We need theorems about `Array.unique/.split` to prove this.
+
+theorem eventSplit_snd_LawfulQueue {exec : Executable net} : 
+  LawfulQueue (exec.eventSplit time).snd time := sorry
+  -- TODO: We need theorems about `Array.unique/.split` to prove this.
+
 private def nextTimerEvents (exec : Executable net) (timers : Array (TimerId net)) (anchor : Time) : Array (Event net) :=
   timers.filterMap fun ⟨reactor, timer⟩ =>
     match exec.reactors reactor |>.timer timer |>.period with
     | none => none
     | some period => return .timer (anchor + period) ⟨reactor, timer⟩
 
+theorem nextTimerEvents_LawfulQueue {exec : Executable net} : 
+  LawfulQueue (exec.nextTimerEvents timers anchor) anchor := sorry
+  -- TODO: We need theorems about `Array.filterMap` to prove this.
+
 structure Next (net : Network) where
-  tag    : Tag
-  events : Array (Event net)
-  queue  : Array (Event net)
+  tag         : Tag
+  events      : Array (Event net)
+  queue       : Array (Event net)
+  lawfulQueue : LawfulQueue queue tag.time
 
 def Next.for (exec : Executable net) : Option (Next net) := 
   match exec.nextTag with 
   | none => none
   | some tag =>
-    let ⟨events, later⟩ := exec.eventSplit tag.time
+    let eventSplit := exec.eventSplit tag.time -- We can't directly destruct here, as this causes problems in the proof of `lawfulQueue`.
+    let events := eventSplit.fst
+    let later := eventSplit.snd
     let timers := events.filterMap (·.timer?)
     let timerEvents := exec.nextTimerEvents timers tag.time
     let queue := later.merge timerEvents
-    some { tag, events, queue }
+    some { tag, events, queue, lawfulQueue := LawfulQueue.merge eventSplit_snd_LawfulQueue nextTimerEvents_LawfulQueue }
 
-theorem Next.lawfulQueue (next : Next net) : LawfulQueue next.queue next.tag.time := sorry
+theorem Next.for_isSome_iff_nextTag_isSome {exec : Executable net} :
+  (Next.for exec).isSome ↔ ¬exec.queue.isEmpty := by
+  simp [Next.for]
+  sorry
+
+theorem Next.for_isSome_iff_queue_not_isEmpty {exec : Executable net} :
+  (Next.for exec).isSome ↔ ¬exec.queue.isEmpty := by
+  sorry
+
+theorem Next.for_preserves_events : ∃ timerEvents, (Next.for exec = some next) → (next.events ++ next.queue) ~ (exec.queue ++ timerEvents) :=
+  sorry
 
 -- The actions-interface for a given reactor according to the `Next` instance.
 def Next.actions (next : Next net) (reactor : ReactorId net) : Interface? (reactor.class.interface .actions) := 
   fun action => 
     match h : next.events.findP? (·.id = .action ⟨reactor, action⟩) with
     | none => none
-    | some event => 
-      have h := Array.findP?_property h
-      event.actionValue (of_decide_eq_true h)
+    | some event => have h := Array.findP?_property h; event.actionValue (of_decide_eq_true h)
 
 end Network.Executable
